Adding to typing proofs in src/Base and src/Expr

src/Base.v
@@ -8,6 +8,7 @@ Export List.ListNotations.
 Open Scope list_scope.
 
 Declare Scope qoreo.
+Create HintDb var_db.
 
 Module Var.
 
@@ -27,6 +28,126 @@ Module Var.
 
   Definition Singleton {A} x a (m : Map.t A) : Prop :=
     Map.Equal m (Map.add x a (Map.empty _)).
+
+  Lemma eq_dec_refl : forall x,
+    eq_dec x x = left (eq_refl x).
+  Proof.
+    intros.
+    induction x; simpl; auto.
+    rewrite IHx; auto.
+  Qed.
+  #[export] Hint Rewrite eq_dec_refl : var_db.
+
+  Lemma remove_add_eq : forall A x (v : A) Gamma,
+    Var.Map.Equal
+      (Var.Map.remove x (Var.Map.add x v Gamma))
+      (Var.Map.remove x Gamma).
+  Proof.
+    intros A x v Gamma y.
+    destruct (eq_dec x y) as [Heq | Hneq].
+    - subst. rewrite MapFacts.F.remove_eq_o; auto.
+      rewrite MapFacts.F.remove_eq_o; auto.
+    - rewrite MapFacts.F.remove_neq_o; auto.
+      rewrite MapFacts.F.add_neq_o; auto.
+      rewrite MapFacts.F.remove_neq_o; auto.
+  Qed.
+  #[export] Hint Rewrite remove_add_eq : var_db. 
+
+  Lemma remove_add_neq : forall A x y (v : A) Gamma,
+    x <> y ->
+    Var.Map.Equal
+      (Var.Map.remove x (Var.Map.add y v Gamma))
+      (Var.Map.add y v (Var.Map.remove x Gamma)).
+  Proof.
+    intros A x y v Gamma Hneq z.
+    destruct (eq_dec x z) as [Heq_xz | Hneq_xz].
+    - subst. rewrite MapFacts.F.remove_eq_o; auto.
+      rewrite MapFacts.F.add_neq_o; auto.
+      rewrite MapFacts.F.remove_eq_o; auto.
+    - rewrite MapFacts.F.remove_neq_o; auto.
+      destruct (eq_dec y z) as [Heq_yz | Hneq_yz].
+      + subst. rewrite MapFacts.F.add_eq_o; auto.
+        rewrite MapFacts.F.add_eq_o; auto.
+      + rewrite MapFacts.F.add_neq_o; auto.
+        rewrite MapFacts.F.add_neq_o; auto.
+        rewrite MapFacts.F.remove_neq_o; auto.
+  Qed.
+  #[export] Hint Rewrite remove_add_neq : var_db.
+
+  Lemma remove_empty : forall A x,
+    Map.Equal (Map.remove x (@Map.empty A))
+      (@Map.empty A).
+  Proof.
+    intros A x y.
+    destruct (eq_dec x y) as [Heq | Hneq].
+    - subst. rewrite MapFacts.F.remove_eq_o; auto.
+    - rewrite MapFacts.F.remove_neq_o; auto.
+  Qed.
+  #[export] Hint Rewrite remove_empty : var_db.
+  
+  Definition concat {A} (m1 m2 : Map.t A) : Map.t A :=
+  Map.fold (fun k v acc => Map.add k v acc) m1 m2.
+
+  Lemma concat_find : forall A (m1 m2 : Map.t A) k,
+    Map.find k (concat m1 m2) =
+    match Map.find k m1 with
+    | Some v => Some v
+    | None => Map.find k m2
+    end.
+  Proof.
+    intros.
+    unfold concat.
+    apply MapFacts.fold_rec; intros.
+    - replace (Map.find k m) with (@None A); auto.
+      {
+        symmetry. apply MapFacts.F.not_find_in_iff.
+        intros [v Hin]. apply (H k v); auto.
+      }
+    - rewrite MapFacts.F.add_o.
+      unfold MapFacts.Add in H1.
+      rewrite H1.
+      rewrite MapFacts.F.add_o.
+      rewrite H2.
+      destruct (Map.E.eq_dec k0 k); auto.
+  Qed.
+
+  Lemma partition_concat : forall A (m m1 m2 : Var.Map.t A),
+    MapFacts.Partition m m1 m2 ->
+    Map.Equal m (concat m1 m2).
+  Proof.
+    intros A m m1 m2 [Hdisj Hpart] x.
+    rewrite concat_find.
+    destruct (Map.find x m) eqn:Hfind.
+    * (* x in dom m *)
+      apply MapFacts.F.find_mapsto_iff in Hfind.
+      apply Hpart in Hfind.
+      destruct Hfind as [Hfind | Hfind].
+      + (* x in dom m1 *)
+        apply MapFacts.F.find_mapsto_iff in Hfind.
+        rewrite Hfind; auto.
+      + (* x in dom m2 *)
+        replace (Map.find x m1) with (@None A).
+        2:{
+          symmetry.
+          apply MapFacts.F.not_find_in_iff.
+          intros Hcontra. apply (Hdisj x). split; auto.
+          eexists; eauto.
+        }
+        symmetry.
+        apply MapFacts.F.find_mapsto_iff; auto.
+    * (* x ∉ m *) 
+      assert (H : Map.find x m1 = None /\ Map.find x m2 = None).
+      {
+        apply MapFacts.F.not_find_in_iff in Hfind.
+          repeat rewrite <- MapFacts.F.not_find_in_iff.
+          split; intros [v Hcontra]; apply Hfind;
+            exists v; apply Hpart; auto.
+      }
+      destruct H as [H1 H2].
+      rewrite H1; rewrite H2.
+      auto.
+  Qed.
+  
 
 End Var.
 
